@prefix : <http://www.exampleThingPrivacyVocabulary.org/2020/sp#> .
@prefix sp: <http://www.exampleThingPrivacyVocabulary.org/2020/sp#> .
@prefix owl: <http://www.w3.org/2002/07/owl#> .
@prefix rdf: <http://www.w3.org/1999/02/22-rdf-syntax-ns#> .
@prefix xml: <http://www.w3.org/XML/1998/namespace> .
@prefix xsd: <http://www.w3.org/2001/XMLSchema#> .
@prefix rdfs: <http://www.w3.org/2000/01/rdf-schema#> .
@prefix 3LConOnt: <http://gessi.lsi.upc.edu/threelevelcontextmodelling/ThreeLContextOnt/UpperLevelOntology> .
@prefix jsonschema: <https://www.w3.org/2019/wot/json-schema#> .
@base <http://www.exampleThingPrivacyVocabulary.org/2020/sp#> .

<http://www.exampleThingPrivacyVocabulary.org/2020/sp#> rdf:type owl:Ontology ;
                                                         rdfs:comment "Situation Privacy vocabulary"^^xsd:string .

#################################################################
#    Annotation properties
#################################################################

###  http://www.exampleThingPrivacyVocabulary.org/2020/sp#Description
sp:Description rdf:type owl:AnnotationProperty .


###  http://www.w3.org/2002/07/owl#maxCardinality
owl:maxCardinality rdf:type owl:AnnotationProperty .


#################################################################
#    Object Properties
#################################################################

###  http://www.exampleThingPrivacyVocabulary.org/2020/sp#bindSituation
sp:bindSituation rdf:type owl:ObjectProperty ;
                 rdfs:domain sp:SituationPrivacyThing ;
                 rdfs:range sp:Situation ;
                 rdfs:comment "IRI : http://www.exampleThingPrivacyVocabulary.org/2020/sp#bindSituation"@nsuri .


###  http://www.exampleThingPrivacyVocabulary.org/2020/sp#conditionType
sp:conditionType rdf:type owl:ObjectProperty ;
                 rdfs:domain sp:PropertyComposition ;
                 rdfs:range sp:ConditionType ;
                 rdfs:comment "IRI : http://www.exampleThingPrivacyVocabulary.org/2020/sp#conditionType"@nsuri .


###  http://www.exampleThingPrivacyVocabulary.org/2020/sp#constraintAssignement
sp:constraintAssignement rdf:type owl:ObjectProperty ;
                         rdfs:domain sp:Privacy ;
                         rdfs:range sp:PrivacyRequirement ;
                         rdfs:comment "IRI : http://www.exampleThingPrivacyVocabulary.org/2020/sp#constraintAssignement"@nsuri .


###  http://www.exampleThingPrivacyVocabulary.org/2020/sp#hasComposedProperties
sp:hasComposedProperties rdf:type owl:ObjectProperty ;
                         rdfs:domain sp:SituationProperties ;
                         rdfs:range sp:PropertyComposition ;
                         rdfs:comment "IRI : http://www.exampleThingPrivacyVocabulary.org/2020/sp#hasComposedProperties"@nsuri .


###  http://www.exampleThingPrivacyVocabulary.org/2020/sp#hasOperationType
sp:hasOperationType rdf:type owl:ObjectProperty ;
                    rdfs:domain sp:Operation ;
                    rdfs:range sp:OperationTypes ;
                    rdfs:comment "IRI : http://www.exampleThingPrivacyVocabulary.org/2020/sp#hasoperationType"@nsuri .


###  http://www.exampleThingPrivacyVocabulary.org/2020/sp#hasProperty
sp:hasProperty rdf:type owl:ObjectProperty ;
               rdfs:domain sp:PropertyComposition ;
               rdfs:range sp:SituationProperties ;
               rdfs:comment "IRI : http://www.exampleThingPrivacyVocabulary.org/2020/sp#hasProperty"@nsuri .


###  http://www.exampleThingPrivacyVocabulary.org/2020/sp#hasPropertyType
sp:hasPropertyType rdf:type owl:ObjectProperty ;
                   rdfs:domain sp:SituationProperties ;
                   rdfs:range jsonschema:DataSchema ;
                   rdfs:comment "IRI : http://www.exampleThingPrivacyVocabulary.org/2020/sp#hasPropertyType"@nsuri .


###  http://www.exampleThingPrivacyVocabulary.org/2020/sp#hasSituationProperties
sp:hasSituationProperties rdf:type owl:ObjectProperty ;
                          rdfs:domain sp:Situation ;
                          rdfs:range sp:SituationProperties ;
                          rdfs:comment "IRI : http://www.exampleThingPrivacyVocabulary.org/2020/sp#hasSituationProperties"@nsuri .


###  http://www.exampleThingPrivacyVocabulary.org/2020/sp#operationAssignement
sp:operationAssignement rdf:type owl:ObjectProperty ;
                        rdfs:domain sp:Privacy ;
                        rdfs:range sp:Operation ;
                        rdfs:comment "IRI : http://www.exampleThingPrivacyVocabulary.org/2020/sp#operationAssignement"@nsuri .


###  http://www.exampleThingPrivacyVocabulary.org/2020/sp#operationExecutor
sp:operationExecutor rdf:type owl:ObjectProperty ;
                     rdfs:domain sp:Operation ;
                     rdfs:range sp:SituationPrivacyThing ;
                     rdfs:comment "IRI : http://www.exampleThingPrivacyVocabulary.org/2020/sp#operationExecutor"@nsuri .


###  http://www.exampleThingPrivacyVocabulary.org/2020/sp#privacyAwareness
sp:privacyAwareness rdf:type owl:ObjectProperty ;
                    rdfs:domain sp:Situation ;
                    rdfs:range sp:Privacy ;
                    rdfs:comment "IRI : http://www.exampleThingPrivacyVocabulary.org/2020/sp#privacyAwareness"@nsuri .


###  http://www.exampleThingPrivacyVocabulary.org/2020/sp#requirementOperation
sp:requirementOperation rdf:type owl:ObjectProperty ;
                        rdfs:domain sp:PrivacyRequirement ;
                        rdfs:range sp:OperationTypes ;
                        rdfs:comment "IRI : http://www.exampleThingPrivacyVocabulary.org/2020/sp#requirementOperation"@nsuri .


###  http://www.exampleThingPrivacyVocabulary.org/2020/sp#requirementThing
sp:requirementThing rdf:type owl:ObjectProperty ;
                    rdfs:domain sp:PrivacyRequirement ;
                    rdfs:range sp:SituationPrivacyThing ;
                    rdfs:comment "IRI : http://www.exampleThingPrivacyVocabulary.org/2020/sp#requirementThing"@nsuri .


###  http://www.exampleThingPrivacyVocabulary.org/2020/sp#requirementsProperties
sp:requirementsProperties rdf:type owl:ObjectProperty ;
                          rdfs:domain sp:PrivacyRequirement ;
                          rdfs:range sp:SituationProperties ;
                          rdfs:comment "IRI : http://www.exampleThingPrivacyVocabulary.org/2020/sp#requirementsProperties"@nsuri .


#################################################################
#    Data properties
#################################################################

###  http://www.exampleThingPrivacyVocabulary.org/2020/sp#logicalOperator
sp:logicalOperator rdf:type owl:DatatypeProperty ;
                   rdfs:domain sp:EEnum ;
                   rdfs:range xsd:integer ;
                   rdfs:isDefinedBy "IRI : http://www.exampleThingPrivacyVocabulary.org/2020/sp#logicalOperator" .


###  http://www.exampleThingPrivacyVocabulary.org/2020/sp#operationName
sp:operationName rdf:type owl:DatatypeProperty ;
                 rdfs:domain sp:Operation ;
                 rdfs:range xsd:string ;
                 rdfs:comment "IRI : http://www.exampleThingPrivacyVocabulary.org/2020/sp#operationName"@nsuri .


###  http://www.exampleThingPrivacyVocabulary.org/2020/sp#operationType
sp:operationType rdf:type owl:DatatypeProperty ;
                 rdfs:domain sp:EEnum ;
                 rdfs:range xsd:string .


###  http://www.exampleThingPrivacyVocabulary.org/2020/sp#propertyName
sp:propertyName rdf:type owl:DatatypeProperty ;
                rdfs:domain sp:SituationProperties ;
                rdfs:range xsd:string ;
                rdfs:comment "IRI : http://www.exampleThingPrivacyVocabulary.org/2020/sp#propertyName"@nsuri .


###  http://www.exampleThingPrivacyVocabulary.org/2020/sp#situationName
sp:situationName rdf:type owl:DatatypeProperty ;
                 rdfs:domain sp:Situation ;
                 rdfs:range xsd:string ;
                 rdfs:comment "IRI : http://www.exampleThingPrivacyVocabulary.org/2020/sp#situationName"@nsuri .


###  http://www.exampleThingPrivacyVocabulary.org/2020/sp#situationPurpose
sp:situationPurpose rdf:type owl:DatatypeProperty ;
                    rdfs:domain sp:Situation ;
                    rdfs:range xsd:string ;
                    rdfs:comment "IRI : http://www.exampleThingPrivacyVocabulary.org/2020/sp#situationPurpose"@nsuri .


###  http://www.exampleThingPrivacyVocabulary.org/2020/sp#thingName
sp:thingName rdf:type owl:DatatypeProperty ;
             rdfs:domain sp:SituationPrivacyThing ;
             rdfs:range xsd:string ;
             rdfs:comment "IRI : http://www.exampleThingPrivacyVocabulary.org/2020/sp#thingName"@nsuri .


#################################################################
#    Classes
#################################################################

###  http://gessi.lsi.upc.edu/threelevelcontextmodelling/ThreeLContextOnt/UpperLevelOntology#ContextInformation
<http://gessi.lsi.upc.edu/threelevelcontextmodelling/ThreeLContextOnt/UpperLevelOntology#ContextInformation> rdf:type owl:Class ;
                                                                                                             owl:equivalentClass sp:Situation .


###  http://www.exampleThingPrivacyVocabulary.org/2020/sp#Class
sp:Class rdf:type owl:Class .


###  http://www.exampleThingPrivacyVocabulary.org/2020/sp#ConditionType
sp:ConditionType rdf:type owl:Class ;
                 owl:equivalentClass [ rdf:type owl:Class ;
                                       owl:oneOf ( sp:ConditionType_and
                                                   sp:ConditionType_or
                                                   sp:ConditionType_xor
                                                 )
                                     ] ;
                 rdfs:subClassOf sp:EEnum ,
                                 [ rdf:type owl:Restriction ;
                                   owl:onProperty sp:conditionType ;
                                   owl:allValuesFrom sp:ConditionType
                                 ] ;
                 rdfs:comment "IRI : http://www.exampleThingPrivcyVocabulary.org/2020/sp#ConditionType"@nsuri .


###  http://www.exampleThingPrivacyVocabulary.org/2020/sp#EEnum
sp:EEnum rdf:type owl:Class .


###  http://www.exampleThingPrivacyVocabulary.org/2020/sp#EPackage
sp:EPackage rdf:type owl:Class .


###  http://www.exampleThingPrivacyVocabulary.org/2020/sp#Operation
sp:Operation rdf:type owl:Class ;
             rdfs:subClassOf sp:Class ;
             rdfs:comment "IRI : http://www.exampleThingPrivcyVocabulary.org/2020/sp#Operation"@nsuri .


###  http://www.exampleThingPrivacyVocabulary.org/2020/sp#OperationTypes
sp:OperationTypes rdf:type owl:Class ;
                  owl:equivalentClass [ rdf:type owl:Class ;
                                        owl:oneOf ( sp:OperationType_collectData
                                                    sp:OperationType_processData
                                                    sp:OperationType_storeData
                                                    sp:OperationType_transferData
                                                  )
                                      ] ;
                  rdfs:subClassOf sp:EEnum ,
                                  [ rdf:type owl:Restriction ;
                                    owl:onProperty sp:hasOperationType ;
                                    owl:allValuesFrom sp:OperationTypes
                                  ] ,
                                  [ rdf:type owl:Restriction ;
                                    owl:onProperty sp:requirementOperation ;
                                    owl:allValuesFrom sp:OperationTypes
                                  ] ;
                  rdfs:comment "IRI : http://www.exampleThingPrivcyVocabulary.org/2020/sp#OperationTypes"@nsuri .


###  http://www.exampleThingPrivacyVocabulary.org/2020/sp#Privacy
sp:Privacy rdf:type owl:Class ;
           rdfs:subClassOf sp:Class ;
           rdfs:comment "IRI : http://www.exampleThingPrivcyVocabulary.org/2020/sp#Privacy"@nsuri .


###  http://www.exampleThingPrivacyVocabulary.org/2020/sp#PrivacyRequirement
sp:PrivacyRequirement rdf:type owl:Class ;
                      rdfs:subClassOf sp:Class ;
                      sp:Description "Describes the requirements of the operation"^^xsd:string ;
                      rdfs:comment "IRI : http://www.exampleThingPrivcyVocabulary.org/2020/sp#PrivacyRequirement"@nsuri .


###  http://www.exampleThingPrivacyVocabulary.org/2020/sp#PropertyComposition
sp:PropertyComposition rdf:type owl:Class ;
                       rdfs:subClassOf sp:Class ;
                       rdfs:comment "IRI : http://www.exampleThingPrivcyVocabulary.org/2020/sp#PropertyCompositon"@nsuri .


###  http://www.exampleThingPrivacyVocabulary.org/2020/sp#Situation
sp:Situation rdf:type owl:Class ;
             rdfs:subClassOf sp:Class ;
             rdfs:comment "IRI : http://www.exampleThingPrivcyVocabulary.org/2020/sp#Situation"@nsuri .


###  http://www.exampleThingPrivacyVocabulary.org/2020/sp#SituationPrivacy
sp:SituationPrivacy rdf:type owl:Class ;
                    rdfs:subClassOf sp:EPackage ;
                    rdfs:comment "http://www.eclipse.org/wot/sp/1.0"@nsuri .


###  http://www.exampleThingPrivacyVocabulary.org/2020/sp#SituationPrivacyThing
sp:SituationPrivacyThing rdf:type owl:Class ;
                         rdfs:subClassOf sp:Class ;
                         rdfs:comment "IRI : http://www.exampleThingPrivcyVocabulary.org/2020/sp#SituationPrivacyThing"@nsuri .


###  http://www.exampleThingPrivacyVocabulary.org/2020/sp#SituationProperties
sp:SituationProperties rdf:type owl:Class ;
                       rdfs:subClassOf sp:Class ;
                       rdfs:comment "IRI : http://www.exampleThingPrivcyVocabulary.org/2020/sp#SituationProperties"@nsuri .


###  https://www.w3.org/2019/wot/json-schema#DataSchema
jsonschema:DataSchema rdf:type owl:Class ;
                      rdfs:subClassOf sp:Class ;
                      rdfs:comment "IRI: https://www.w3.org/2019/wot/json-schema#DataSchema"@nsuri .


#################################################################
#    Individuals
#################################################################

###  http://www.exampleThingPrivacyVocabulary.org/2020/sp#ConditionType_and
sp:ConditionType_and rdf:type owl:NamedIndividual ,
                              sp:ConditionType ;
                     sp:logicalOperator "0"^^xsd:int ;
                     sp:operationType "and" .


###  http://www.exampleThingPrivacyVocabulary.org/2020/sp#ConditionType_or
sp:ConditionType_or rdf:type owl:NamedIndividual ,
                             sp:ConditionType ;
                    sp:logicalOperator "1"^^xsd:int ;
                    sp:operationType "or" .


###  http://www.exampleThingPrivacyVocabulary.org/2020/sp#ConditionType_xor
sp:ConditionType_xor rdf:type owl:NamedIndividual ,
                              sp:ConditionType ;
                     sp:logicalOperator "2"^^xsd:int ;
                     sp:operationType "xor" .


###  http://www.exampleThingPrivacyVocabulary.org/2020/sp#OperationType_collectData
sp:OperationType_collectData rdf:type owl:NamedIndividual ,
                                      sp:OperationTypes ;
                             sp:logicalOperator "1"^^xsd:int ;
                             sp:operationType "collectData" .


###  http://www.exampleThingPrivacyVocabulary.org/2020/sp#OperationType_processData
sp:OperationType_processData rdf:type owl:NamedIndividual ,
                                      sp:OperationTypes ;
                             sp:logicalOperator "3"^^xsd:int ;
                             sp:operationType "processData" .


###  http://www.exampleThingPrivacyVocabulary.org/2020/sp#OperationType_storeData
sp:OperationType_storeData rdf:type owl:NamedIndividual ,
                                    sp:OperationTypes ;
                           sp:logicalOperator "0"^^xsd:int ;
                           sp:operationType "storeData" .


###  http://www.exampleThingPrivacyVocabulary.org/2020/sp#OperationType_transferData
sp:OperationType_transferData rdf:type owl:NamedIndividual ,
                                       sp:OperationTypes ;
                              sp:logicalOperator "2"^^xsd:int ;
                              sp:operationType "transferData" .


###  http://www.exampleThingPrivacyVocabulary.org/2020/sp#SituationPrivacyThing_HvqjEDGhEeukprZNUg_xuw
sp:SituationPrivacyThing_HvqjEDGhEeukprZNUg_xuw rdf:type owl:NamedIndividual .


[ owl:maxCardinality "1"^^xsd:int
] .

[ owl:maxCardinality "1"^^xsd:int
 ] .

[ owl:maxCardinality "1"^^xsd:int
 ] .

[ owl:maxCardinality "1"^^xsd:int
 ] .

[ owl:maxCardinality "1"^^xsd:int
 ] .

###  Generated by the OWL API (version 4.5.9.2019-02-01T07:24:44Z) https://github.com/owlcs/owlapi
